src/Reflection/MapCastWithCastOp.v
@@ -1,0 +1,130 @@
+Require Import Crypto.Reflection.Syntax.
+Require Import Crypto.Reflection.Application.
+Require Import Crypto.Reflection.MapCast.
+Require Import Crypto.Util.Sigma.
+Require Import Crypto.Util.Prod.
+Require Import Crypto.Util.Option.
+
+Local Open Scope ctype_scope.
+Local Open Scope expr_scope.
+Section language.
+  Context {base_type_code1 base_type_code2 : Type}
+          {interp_base_type1 : base_type_code1 -> Type}
+          {interp_base_type2 : base_type_code2 -> Type}
+          {op1 : flat_type base_type_code1 -> flat_type base_type_code1 -> Type}
+          {op2 : flat_type base_type_code2 -> flat_type base_type_code2 -> Type}
+          (interp_op2 : forall src dst, op2 src dst -> interp_flat_type interp_base_type2 src -> interp_flat_type interp_base_type2 dst)
+          (base_type_code1_beq : base_type_code1 -> base_type_code1 -> bool)
+          (base_type_code1_bl : forall x y, base_type_code1_beq x y = true -> x = y)
+          (base_type_code1_lb : forall x y, x = y -> base_type_code1_beq x y = true)
+          (failv : forall {t}, interp_base_type1 t)
+          (new_base_type : forall t, interp_base_type2 t -> base_type_code1)
+          (transfer_base_const : forall t1 t2 (x1 : interp_base_type1 t1) (x2 : interp_base_type2 t2),
+              interp_base_type1 (new_base_type t2 x2))
+          (Cast : forall var t1 t2, @exprf base_type_code1 interp_base_type1 op1 var (Tbase t1)
+                                    -> @exprf base_type_code1 interp_base_type1 op1 var (Tbase t2))
+          (is_cast : forall t1 t2, op1 t1 t2 -> bool).
+  Local Notation new_flat_type (*: forall t, interp_flat_type interp_base_type2 t -> flat_type base_type_code1*)
+    := (@SmartFlatTypeMap2 _ _ interp_base_type2 (fun t v => Tbase (new_base_type t v))).
+  Local Notation new_type := (@new_type base_type_code1 base_type_code2 interp_base_type2 new_base_type).
+  Context (new_op : forall ovar src1 dst1 src2 dst2 (opc1 : op1 src1 dst1) (opc2 : op2 src2 dst2)
+                             args2,
+              option { new_src : _ & (@exprf base_type_code1 interp_base_type1 op1 ovar new_src
+                                      -> @exprf base_type_code1 interp_base_type1 op1 ovar (new_flat_type (interpf interp_op2 (Op opc2 args2))))%type }).
+
+  Fixpoint VarBound {var} T1 T2 : interp_flat_type var T1 -> exprf _ interp_base_type1 op1 (var:=var) T2
+    := match T1, T2 return interp_flat_type var T1 -> exprf _ _ _ T2 with
+       | Tbase T1', Tbase T2' => fun v : var T1' => Cast _ _ _ (Var v)
+       | Prod A1 B1, Prod A2 B2
+         => fun xy
+            => Pair (@VarBound _ _ _ (fst xy)) (@VarBound _ _ _ (snd xy))
+       | Tbase _, _
+       | Prod _ _, _
+         => fun _ => Const (SmartValf _ (@failv) _)
+       end.
+  Fixpoint SmartBound {var t1 t2} (v : @exprf _ interp_base_type1 op1 var t1) : @exprf _ interp_base_type1 op1 var t2.
+  Proof.
+    refine match Sumbool.sumbool_of_bool (flat_type_beq _ base_type_code1_beq t1 t2) with
+           | left pf => match flat_type_dec_bl _ _ base_type_code1_bl _ _ pf in (_ = y) return exprf _ _ _ y with
+                        | eq_refl => v
+                        end
+           | right _ => _
+           end.
+    refine (match v in exprf _ _ _ t1, t2 return (exprf _ _ _ _ -> exprf _ _ _ t2) -> exprf _ _ _ t2 with
+            | Op t1 tR opc args, _
+              => if is_cast _ _ opc
+                 then fun _ => @SmartBound _ _ _ args
+                 else fun default => default v
+            | Pair _ ex _ ey, Prod _ _ => fun _ => Pair (@SmartBound _ _ _ ex) (@SmartBound _ _ _ ey)
+            | v', _ => fun default => default v'
+            end _).
+    refine (match t1, t2 return exprf _ _ _ t1 -> exprf _ _ _ t2 with
+            | Tbase t1', Tbase t2' => Cast _ _ _
+            | Prod A1 B1, Prod A2 B2 => fun x => LetIn x (VarBound _ _)
+            | Tbase _, _
+            | Prod _ _, _
+              => fun _ => Const (SmartValf _ (@failv) _)
+            end).
+  Defined.
+  Definition bound_op ovar
+             {src1 dst1 src2 dst2}
+             (opc1 : op1 src1 dst1)
+             (opc2 : op2 src2 dst2)
+    : forall args2
+             (args' : @exprf base_type_code1 interp_base_type1 op1 ovar (@new_flat_type _ (interpf interp_op2 args2))),
+      @exprf base_type_code1 interp_base_type1 op1 ovar (@new_flat_type _ (interpf interp_op2 (Op opc2 args2)))
+    := if is_cast _ _ opc1
+       then fun _ x => SmartBound x
+       else fun args2 args'
+            => match new_op _ _ _ _ _ opc1 opc2 args2 with
+               | Some f => projT2 f (SmartBound args')
+               | None => Const (SmartValf _ (@failv) _)
+               end.
+
+  Section with_var.
+    Context {ovar : base_type_code1 -> Type}.
+    Local Notation ivar t := (@exprf base_type_code1 interp_base_type1 op1 ovar (Tbase t)) (only parsing).
+    Local Notation ivarf := (fun t => ivar t).
+
+    Fixpoint bound_var tx1 tx2 tC1
+             {struct tx2}
+      : forall (f : interp_flat_type ivarf tx1 -> exprf _ interp_base_type1 op1 (var:=ovar) tC1)
+               (v : interp_flat_type ivarf tx2),
+        exprf _ interp_base_type1 op1 (var:=ovar) tC1
+      := match tx1, tx2 return (interp_flat_type _ tx1 -> _) -> interp_flat_type _ tx2 -> _ with
+         | Tbase T1, Tbase T2 => fun f v => f (SmartBound v)
+         | Prod A1 B1, Prod A2 B2
+           => fun f v
+              => @bound_var
+                   _ _ _
+                   (fun v1 => @bound_var _ _ _ (fun v2 => f (v1, v2)%core) (snd v))
+                   (fst v)
+         | Tbase _, _
+         | Prod _ _, _
+           => fun f _ => f (SmartValf _ (fun t => Const (t:=Tbase _) (@failv t)) _)
+         end.
+
+    Definition mapf_interp_cast_with_cast_op
+               {t1} (e1 : @exprf base_type_code1 interp_base_type1 op1 ivarf t1)
+               {t2} (e2 : @exprf base_type_code2 interp_base_type2 op2 interp_base_type2 t2)
+      : @exprf base_type_code1 interp_base_type1 op1 ovar (@new_flat_type _ (interpf interp_op2 e2))
+      := @mapf_interp_cast
+           base_type_code1 base_type_code2 interp_base_type1 interp_base_type2 op1 op2
+           interp_op2 (@failv) new_base_type transfer_base_const bound_op
+           ovar bound_var
+           t1 e1 t2 e2.
+    Definition map_interp_cast_with_cast_op
+             {t1} (e1 : @expr base_type_code1 interp_base_type1 op1 ivarf t1)
+             {t2} (e2 : @expr base_type_code2 interp_base_type2 op2 interp_base_type2 t2)
+      : forall (args2 : interp_all_binders_for' t2 interp_base_type2),
+        @expr base_type_code1 interp_base_type1 op1 ovar (@new_type _ args2 (interp interp_op2 e2))
+      := @map_interp_cast
+           base_type_code1 base_type_code2 interp_base_type1 interp_base_type2 op1 op2
+           interp_op2 (@failv) new_base_type transfer_base_const bound_op
+           ovar bound_var
+           t1 e1 t2 e2.
+  End with_var.
+End language.
+
+Global Arguments mapf_interp_cast_with_cast_op {_ _ _ _ _ _ _} base_type_code1_beq base_type_code1_bl failv {_} transfer_base_const Cast is_cast new_op {ovar} {t1} e1 {t2} e2.
+Global Arguments map_interp_cast_with_cast_op {_ _ _ _ _ _ _} base_type_code1_beq base_type_code1_bl failv {_} transfer_base_const Cast is_cast new_op {ovar} {t1} e1 {t2} e2 args2.
